%==========================================================
\section{Exercise 1}\label{sec:ex1}
%==========================================================
Show that 
\begin{align*}
    \quad \frac{\partial (\mathbf{a}^{T}\mathbf{x})}{\partial \mathbf{x}} &= \mathbf{a}^{T} && \text{and} & \frac{\partial (\mathbf{a}^{T} \mathbf{A} \mathbf{a})}{\partial \mathbf{a}} &= \mathbf{a}^{T} (\mathbf{A} \mathbf{A}^{T}) && \text{and} & \frac{\partial (\mathbf{x} - \mathbf{A} \mathbf{s})^{T} (\mathbf{x} - \mathbf{A} \mathbf{s})}{\partial \mathbf{s}} &= -2 (\mathbf{x} - \mathbf{A} \mathbf{s})^{T} \mathbf{A}
\end{align*}

\begin{figure}
    \centering
    \includegraphics[width=0.8\linewidth, angle=270]{latex/figures/ex1.jpeg}
    \caption{Answer for exercise 1}
    \label{fig:ex1}
\end{figure}